Add support for preconditions and postconditions

byteback-annotations/src/main/java/byteback/annotations/Contract.java
@@ -10,55 +10,55 @@ import java.lang.annotation.Target;
  */
 public interface Contract {
 
-  /**
-   * Declares a predicate method.
-   *
-   * A predicate method is a completely pure static method containing boolean
-   * statements verifying conditions on its inputs. A predicate method may only
-   * indirectly call other static predicate methods.
-   * <p>
-   * There could possibly be exceptions for certain virtual or interface calls
-   * needed for the specification of quantifiers.
-   * <p>
-   * TODO: delineate such exceptions here.
-   */
-  @Retention(RetentionPolicy.RUNTIME)
-  @Target({ ElementType.METHOD })
-  public static @interface Pure {
-  }
+	/**
+	 * Declares a predicate method.
+	 *
+	 * A predicate method is a completely pure static method containing boolean
+	 * statements verifying conditions on its inputs. A predicate method may only
+	 * indirectly call other static predicate methods.
+	 * <p>
+	 * There could possibly be exceptions for certain virtual or interface calls
+	 * needed for the specification of quantifiers.
+	 * <p>
+	 * TODO: delineate such exceptions here.
+	 */
+	@Retention(RetentionPolicy.RUNTIME)
+	@Target({ElementType.METHOD})
+	public static @interface Pure {
+	}
 
-  /**
-   * Declares that the function is already defined in the preamble.
-   */
-  @Retention(RetentionPolicy.RUNTIME)
-  @Target({ ElementType.METHOD })
-  public static @interface Prelude {
-    public String value();
-  }
+	/**
+	 * Declares that the function is already defined in the preamble.
+	 */
+	@Retention(RetentionPolicy.RUNTIME)
+	@Target({ElementType.METHOD})
+	public static @interface Prelude {
+		public String value();
+	}
 
-  @Retention(RetentionPolicy.RUNTIME)
-  @Target({ ElementType.METHOD })
-  public static @interface Require {
-    public String value();
-  }
+	@Retention(RetentionPolicy.RUNTIME)
+	@Target({ElementType.METHOD})
+	public static @interface Require {
+		public String value();
+	}
 
-  @Retention(RetentionPolicy.RUNTIME)
-  @Target({ ElementType.METHOD })
-  public static @interface Ensure {
-    public String value();
-  }
+	@Retention(RetentionPolicy.RUNTIME)
+	@Target({ElementType.METHOD})
+	public static @interface Ensure {
+		public String value();
+	}
 
-  /**
-   * Declares a condition method.
-   * <p>
-   * Condition methods can be used to represent preconditions, postconditions or
-   * invariants. Every condition method must be both, static and pure. The return
-   * type of the annotated method must be void, as conditions are enforced by
-   * means of assertions. A condition method may only call predicate methods.
-   */
-    @Retention(RetentionPolicy.RUNTIME)
-    @Target({ ElementType.METHOD })
-    public static @interface Condition {
-    }
+	/**
+	 * Declares a condition method.
+	 * <p>
+	 * Condition methods can be used to represent preconditions, postconditions or
+	 * invariants. Every condition method must be both, static and pure. The return
+	 * type of the annotated method must be void, as conditions are enforced by
+	 * means of assertions. A condition method may only call predicate methods.
+	 */
+	@Retention(RetentionPolicy.RUNTIME)
+	@Target({ElementType.METHOD})
+	public static @interface Condition {
+	}
 
 }
