byteback-annotations/src/main/java/byteback/annotations/Operator.java
@@ -12,165 +12,177 @@ import byteback.annotations.Contract.Pure;
  */
 public interface Operator {
 
-    /**
-     * Boolean implication.
-     * 
-     * @param a Antecedent of the implication.
-     * @param b Consequent of the implication.
-     * @return {@code true} if {@code a -> b}.
-     */
-    @Pure
-    @Prelude("implies")
-    public static boolean implies(final boolean a, final boolean b) {
-        return !a || b;
-    }
+	/**
+	 * Boolean implication.
+	 * 
+	 * @param a
+	 *            Antecedent of the implication.
+	 * @param b
+	 *            Consequent of the implication.
+	 * @return {@code true} if {@code a -> b}.
+	 */
+	@Pure
+	@Prelude("implies")
+	public static boolean implies(final boolean a, final boolean b) {
+		return !a || b;
+	}
 
-    /**
-     * Boolean equivalence.
-     * 
-     * @param a First statement.
-     * @param b Second statement.
-     * @return {@code true} if {@code a <-> b}.
-     */
-    @Pure
-    @Prelude("iff")
-    public static boolean iff(final boolean a, final boolean b) {
-        return a == b;
-    }
+	/**
+	 * Boolean equivalence.
+	 * 
+	 * @param a
+	 *            First statement.
+	 * @param b
+	 *            Second statement.
+	 * @return {@code true} if {@code a <-> b}.
+	 */
+	@Pure
+	@Prelude("iff")
+	public static boolean iff(final boolean a, final boolean b) {
+		return a == b;
+	}
 
-    /**
-     * Boolean AND.
-     *
-     * @param a First operand.
-     * @param b Second operand.
-     * @return {@code true} if {@code a && b}.
-     */
-    @Pure
-    @Prelude("and")
-    public static boolean and(final boolean a, final boolean b) {
-        return a && b;
-    }
+	/**
+	 * Boolean AND.
+	 *
+	 * @param a
+	 *            First operand.
+	 * @param b
+	 *            Second operand.
+	 * @return {@code true} if {@code a && b}.
+	 */
+	@Pure
+	@Prelude("and")
+	public static boolean and(final boolean a, final boolean b) {
+		return a && b;
+	}
 
-    /**
-     * Boolean OR.
-     *
-     * @param a First operand.    
-     * @param b Second operand.
-     * @return {@code true} if {@code a || b}.
-     */
-    @Pure
-    @Prelude("or")
-    public static boolean or(final boolean a, final boolean b) {
-        return a || b;
-    }
+	/**
+	 * Boolean OR.
+	 *
+	 * @param a
+	 *            First operand.
+	 * @param b
+	 *            Second operand.
+	 * @return {@code true} if {@code a || b}.
+	 */
+	@Pure
+	@Prelude("or")
+	public static boolean or(final boolean a, final boolean b) {
+		return a || b;
+	}
 
-    /**
-     * Boolean NOT.
-     *
-     * @param a Single operand.    
-     * @return {@code true} if {@code !o}.
-     */
-    @Pure
-    @Prelude("not")
-    public static boolean not(final boolean a) {
-        return !a;
-    }
+	/**
+	 * Boolean NOT.
+	 *
+	 * @param a
+	 *            Single operand.
+	 * @return {@code true} if {@code !o}.
+	 */
+	@Pure
+	@Prelude("not")
+	public static boolean not(final boolean a) {
+		return !a;
+	}
 
-    /**
-     * Object equality.
-     *
-     * @param a First operand.    
-     * @param b Second operand.
-     * @return {@code true} if {@code a || b}.
-     */
-    @Pure
-    @Prelude("eq")
-    public static boolean eq(final Object a, final Object b) {
-        return a.equals(b);
-    }
+	/**
+	 * Object equality.
+	 *
+	 * @param a
+	 *            First operand.
+	 * @param b
+	 *            Second operand.
+	 * @return {@code true} if {@code a || b}.
+	 */
+	@Pure
+	@Prelude("eq")
+	public static boolean eq(final Object a, final Object b) {
+		return a.equals(b);
+	}
 
-    /**
-     * Equality overloaded for boolean types to avoid auto-boxing of booleans.
-     */
-    @Pure
-    @Prelude("eq")
-    public static boolean eq(final boolean a, final boolean b) {
-        return a == b;
-    }
+	/**
+	 * Equality overloaded for boolean types to avoid auto-boxing of booleans.
+	 */
+	@Pure
+	@Prelude("eq")
+	public static boolean eq(final boolean a, final boolean b) {
+		return a == b;
+	}
 
-    /**
-     * Equality overloaded for byte types to avoid auto-boxing of bytes.
-     */
-    @Pure
-    @Prelude("eq")
-    public static boolean eq(final byte a, final byte b) {
-        return a == b;
-    }
+	/**
+	 * Equality overloaded for byte types to avoid auto-boxing of bytes.
+	 */
+	@Pure
+	@Prelude("eq")
+	public static boolean eq(final byte a, final byte b) {
+		return a == b;
+	}
 
-    /**
-     * Equality overloaded for int types to avoid auto-boxing of integers.
-     */
-    @Pure
-    @Prelude("eq")
-    public static boolean eq(final int a, final int b) {
-        return a == b;
-    }
+	/**
+	 * Equality overloaded for int types to avoid auto-boxing of integers.
+	 */
+	@Pure
+	@Prelude("eq")
+	public static boolean eq(final int a, final int b) {
+		return a == b;
+	}
 
-    /**
-     * Equality overloaded for boolean types to avoid auto-boxing of booleans.
-     */
-    @Pure
-    @Prelude("eq")
-    public static boolean eq(final char a, final char b) {
-        return a == b;
-    }
+	/**
+	 * Equality overloaded for boolean types to avoid auto-boxing of booleans.
+	 */
+	@Pure
+	@Prelude("eq")
+	public static boolean eq(final char a, final char b) {
+		return a == b;
+	}
 
-    /**
-     * Equality overloaded for double types to avoid auto-boxing of doubles.
-     */
-    @Pure
-    @Prelude("eq")
-    public static boolean eq(final double a, final double b) {
-        return a == b;
-    }
+	/**
+	 * Equality overloaded for double types to avoid auto-boxing of doubles.
+	 */
+	@Pure
+	@Prelude("eq")
+	public static boolean eq(final double a, final double b) {
+		return a == b;
+	}
 
-    /**
-     * Equality overloaded for float types to avoid auto-boxing of floats.
-     */
-    @Pure
-    @Prelude("eq")
-    public static boolean eq(final float a, final float b) {
-        return a == b;
-    }
+	/**
+	 * Equality overloaded for float types to avoid auto-boxing of floats.
+	 */
+	@Pure
+	@Prelude("eq")
+	public static boolean eq(final float a, final float b) {
+		return a == b;
+	}
 
-    /**
-     * Equality overloaded for long types to avoid auto-boxing of longs.
-     */
-    @Pure
-    @Prelude("eq")
-    public static boolean eq(final long a, final long b) {
-        return a == b;
-    }
+	/**
+	 * Equality overloaded for long types to avoid auto-boxing of longs.
+	 */
+	@Pure
+	@Prelude("eq")
+	public static boolean eq(final long a, final long b) {
+		return a == b;
+	}
 
-    /**
-     * Equality overloaded for short types to avoid auto-boxing of shorts.
-     */
-    @Pure
-    @Prelude("eq")
-    public static boolean eq(final short a, final short b) {
-        return a == b;
-    }
+	/**
+	 * Equality overloaded for short types to avoid auto-boxing of shorts.
+	 */
+	@Pure
+	@Prelude("eq")
+	public static boolean eq(final short a, final short b) {
+		return a == b;
+	}
 
-    /**
-     * Specifies a reference to a old expression in a condition.
-     * <p>
-     * This expression is only allowed in the specification of conditions.
-     *
-     * @param a Single operand.
-     * @return The given {@code a} instance.
-     */
-    public static <T> T old(T a) {
-        return a;
-    }
+	/**
+	 * Specifies a reference to a old expression in a condition.
+	 * <p>
+	 * This expression is only allowed in the specification of conditions.
+	 *
+	 * @param a
+	 *            Single operand.
+	 * @return The given {@code a} instance.
+	 */
+	public static <T> T old(T a) {
+		return a;
+	}
 
 }
