byteback-annotations/src/main/java/byteback/annotations/Quantifier.java
@@ -7,41 +7,47 @@ import java.util.function.Predicate;
  */
 public interface Quantifier {
 
-    /**
-     * Existential quantifier.
-     * 
-     * @param d   The domain of discourse.
-     * @param p   The predicate applied to the domain.
-     * @param <T> Type of the iterated elements.
-     * @return {@code true} if there is a term in {@code d} that satisfies
-     *         {@code p}.
-     */
-    public static <T> boolean exists(final Iterable<T> d, final Predicate<T> p) {
-        for (T x : d) {
-            if (p.test(x)) {
-                return true;
-            }
-        }
+	/**
+	 * Existential quantifier.
+	 * 
+	 * @param d
+	 *            The domain of discourse.
+	 * @param p
+	 *            The predicate applied to the domain.
+	 * @param <T>
+	 *            Type of the iterated elements.
+	 * @return {@code true} if there is a term in {@code d} that satisfies
+	 *         {@code p}.
+	 */
+	public static <T> boolean exists(final Iterable<T> d, final Predicate<T> p) {
+		for (T x : d) {
+			if (p.test(x)) {
+				return true;
+			}
+		}
 
-        return false;
-    }
+		return false;
+	}
 
-    /**
-     * Universal quantifier.
-     * 
-     * @param d   The domain of discourse.
-     * @param p   The predicate applied to the domain.
-     * @param <T> Type of the iterated elements.
-     * @return {@code true} if all terms in {@code d} satisfy {@code p}.
-     */
-    public static <T> boolean forAll(final Iterable<T> d, final Predicate<T> p) {
-        for (T x : d) {
-            if (!p.test(x)) {
-                return false;
-            }
-        }
+	/**
+	 * Universal quantifier.
+	 * 
+	 * @param d
+	 *            The domain of discourse.
+	 * @param p
+	 *            The predicate applied to the domain.
+	 * @param <T>
+	 *            Type of the iterated elements.
+	 * @return {@code true} if all terms in {@code d} satisfy {@code p}.
+	 */
+	public static <T> boolean forAll(final Iterable<T> d, final Predicate<T> p) {
+		for (T x : d) {
+			if (!p.test(x)) {
+				return false;
+			}
+		}
 
-        return true;
-    }
+		return true;
+	}
 
 }
