byteback-core/src/main/java/byteback/core/converter/soot/boogie/ProcedureConverter.java
@@ -1,19 +1,30 @@
 package byteback.core.converter.soot.boogie;
 
+import byteback.core.representation.soot.annotation.SootAnnotationElement.StringElementExtractor;
 import byteback.core.representation.soot.type.SootType;
 import byteback.core.representation.soot.type.SootTypeVisitor;
 import byteback.core.representation.soot.unit.SootMethodUnit;
+import byteback.frontend.boogie.ast.Accessor;
 import byteback.frontend.boogie.ast.Body;
 import byteback.frontend.boogie.ast.BoundedBinding;
+import byteback.frontend.boogie.ast.Expression;
 import byteback.frontend.boogie.ast.Label;
+import byteback.frontend.boogie.ast.List;
+import byteback.frontend.boogie.ast.PostCondition;
+import byteback.frontend.boogie.ast.PreCondition;
 import byteback.frontend.boogie.ast.ProcedureDeclaration;
 import byteback.frontend.boogie.ast.ProcedureSignature;
+import byteback.frontend.boogie.ast.Specification;
 import byteback.frontend.boogie.ast.TypeAccess;
+import byteback.frontend.boogie.ast.ValueReference;
 import byteback.frontend.boogie.builder.BoundedBindingBuilder;
 import byteback.frontend.boogie.builder.ProcedureDeclarationBuilder;
 import byteback.frontend.boogie.builder.ProcedureSignatureBuilder;
 import byteback.frontend.boogie.builder.VariableDeclarationBuilder;
+import java.util.Collection;
 import java.util.Map;
+import java.util.stream.Stream;
+import soot.BooleanType;
 import soot.Local;
 import soot.Type;
 import soot.Unit;
@@ -53,7 +64,7 @@ public class ProcedureConverter {
 			@Override
 			public void caseDefault(final Type type) {
 				final TypeAccess typeAccess = new TypeAccessExtractor().visit(methodUnit.getReturnType());
-        final BoundedBinding binding = Prelude.getReturnBindingBuilder().typeAccess(typeAccess).build();
+				final BoundedBinding binding = Prelude.getReturnBindingBuilder().typeAccess(typeAccess).build();
 				signatureBuilder.addOutputBinding(binding);
 			}
 
@@ -75,13 +86,56 @@ public class ProcedureConverter {
 		return body;
 	}
 
+	public static Stream<Expression> makeConditions(final SootMethodUnit methodUnit, final String annotation) {
+		final Stream<String> sourceNames = methodUnit.getAnnotationValues(annotation)
+				.map((element) -> new StringElementExtractor().visit(element));
+		final List<Expression> arguments = makeArguments(methodUnit);
+
+		return sourceNames.map((sourceName) -> makeCondition(methodUnit, sourceName, arguments));
+	}
+
+	public static Expression makeCondition(final SootMethodUnit target, final String sourceName,
+			final List<Expression> arguments) {
+
+		final Collection<SootType> parameterTypes = target.getParameterTypes();
+		parameterTypes.add(target.getReturnType());
+		final SootType returnType = new SootType(BooleanType.v());
+		final SootMethodUnit source = target.getClassUnit().getMethodUnit(sourceName, parameterTypes, returnType).get();
+
+		return ConditionManager.instance().convert(source).getFunction().inline(arguments);
+	}
+
+	public static List<Expression> makeArguments(final SootMethodUnit methodUnit) {
+		final List<Expression> references = new List<>(Prelude.getHeapVariable().getValueReference());
+
+		for (Local local : methodUnit.getBody().getParameterLocals()) {
+			references.add(new ValueReference(new Accessor(local.getName())));
+		}
+
+		references.add(Prelude.getReturnValueReference());
+
+		return references;
+	}
+
+	public static List<Specification> makeSpecifications(final SootMethodUnit methodUnit) {
+		final Stream<Specification> preconditions = makeConditions(methodUnit,
+				"Lbyteback/annotations/Contract$Require;").map((expression) -> new PreCondition(false, expression));
+		final Stream<Specification> postconditions = makeConditions(methodUnit,
+				"Lbyteback/annotations/Contract$Ensure;").map((expression) -> new PostCondition(false, expression));
+		final Iterable<Specification> specifications = Stream.concat(preconditions, postconditions)::iterator;
+
+		return new List<Specification>().addAll(specifications);
+	}
+
 	public ProcedureDeclaration convert(final SootMethodUnit methodUnit) {
 		final ProcedureDeclarationBuilder procedureBuilder = new ProcedureDeclarationBuilder();
 		final ProcedureSignature signature = makeSignature(methodUnit);
+		final List<Specification> specifications = makeSpecifications(methodUnit);
 		final Body body = makeBody(methodUnit);
 		procedureBuilder.name(NameConverter.methodName(methodUnit));
 		procedureBuilder.signature(signature);
 		procedureBuilder.body(body);
+		procedureBuilder.specification(specifications);
 
 		return procedureBuilder.build();
 	}
