byteback-core/src/main/java/byteback/core/representation/soot/unit/SootMethodUnit.java
@@ -1,18 +1,48 @@
 package byteback.core.representation.soot.unit;
 
 import byteback.core.representation.soot.annotation.SootAnnotation;
+import byteback.core.representation.soot.annotation.SootAnnotationElement;
 import byteback.core.representation.soot.body.SootBody;
 import byteback.core.representation.soot.type.SootType;
+import java.util.Collection;
 import java.util.Iterator;
 import java.util.List;
 import java.util.Optional;
 import java.util.stream.Collectors;
 import java.util.stream.Stream;
 import soot.SootMethod;
-import soot.Type;
 import soot.tagkit.VisibilityAnnotationTag;
 
 public class SootMethodUnit {
+
+	static String formatSignature(final String name, final Collection<SootType> parameterTypes,
+			final SootType returnType) {
+		final StringBuilder builder = new StringBuilder();
+		builder.append(returnType);
+		builder.append(" ");
+		builder.append(name);
+		builder.append(formatParameters(parameterTypes));
+
+		return builder.toString();
+	}
+
+	static String formatParameters(final Collection<SootType> parameterTypes) {
+		final StringBuilder builder = new StringBuilder();
+		final Iterator<SootType> iterator = parameterTypes.iterator();
+		builder.append("(");
+
+		while (iterator.hasNext()) {
+			builder.append(iterator.next().toString());
+
+			if (iterator.hasNext()) {
+				builder.append(",");
+			}
+		}
+
+		builder.append(")");
+
+		return builder.toString();
+	}
 
 	private final SootMethod sootMethod;
 
@@ -32,19 +62,8 @@ public class SootMethodUnit {
 
 	public String getIdentifier() {
 		final StringBuilder builder = new StringBuilder();
-		final Iterator<Type> typeIterator = sootMethod.getParameterTypes().iterator();
 		builder.append(getName());
-		builder.append("(");
-
-		while (typeIterator.hasNext()) {
-			builder.append(typeIterator.next().toString());
-
-			if (typeIterator.hasNext()) {
-				builder.append(",");
-			}
-		}
-
-		builder.append(")");
+		builder.append(formatParameters(getParameterTypes()));
 
 		return builder.toString();
 	}
@@ -66,7 +85,23 @@ public class SootMethodUnit {
 	}
 
 	public Optional<SootAnnotation> getAnnotation(final String type) {
-		return annotations().filter((tag) -> tag.getTypeName().equals(type)).findFirst();
+		return getAnnotations(type).findFirst();
+	}
+
+	public Stream<SootAnnotation> getAnnotations(final String type) {
+		return annotations().filter((tag) -> tag.getTypeName().equals(type));
+	}
+
+	public Stream<SootAnnotationElement> getAnnotationValues(final String type) {
+		return getAnnotations(type).flatMap((annotation) -> {
+			final Optional<SootAnnotationElement> element = annotation.getValue();
+
+			if (element.isPresent()) {
+				return Stream.of(element.get());
+			} else {
+				return Stream.empty();
+			}
+		});
 	}
 
 	public Stream<SootAnnotation> annotations() {
