byteback-dummy/java8/src/main/java/byteback/dummy/condition/Simple.java
@@ -1,28 +1,30 @@
 package byteback.dummy.condition;
 
+import static byteback.annotations.Operator.eq;
+
 import byteback.annotations.Contract.Condition;
 import byteback.annotations.Contract.Ensure;
 
 public class Simple {
 
-  @Condition
-  public static boolean returns_1(int returns) {
-    return returns == 1;
-  }
+	@Condition
+	public static boolean returns_1(int returns) {
+		return eq(returns, 1);
+	}
 
-  @Condition
-  public static boolean returns_argument(int a, int returns) {
-    return returns == a;
-  }
+	@Condition
+	public static boolean returns_argument(int a, int returns) {
+		return eq(returns, a);
+	}
 
-  @Ensure("returns_1")
-  public static int returnsOne() {
-    return 1;
-  }
+	@Ensure("returns_1")
+	public static int returnsOne() {
+		return 1;
+	}
 
-  @Ensure("returns_argument")
-  public static int identity(int a) {
-    return a;
-  }
+	@Ensure("returns_argument")
+	public static int identity(int a) {
+		return a;
+	}
 
 }
