byteback-frontend/boogie/src/test/java/byteback/frontend/boogie/ResourcesUtil.java
@@ -13,49 +13,49 @@ import java.nio.file.Paths;
  */
 public class ResourcesUtil {
 
-  /**
-   * Base path to the resource folder.
-   */
-  final private static Path resourcesPath = Paths.get("src", "test", "resources");
+	/**
+	 * Base path to the resource folder.
+	 */
+	final private static Path resourcesPath = Paths.get("src", "test", "resources");
 
-  /**
-   * Base path to the Boogie resource folder.
-   */
-  final private static Path boogiePath = resourcesPath.resolve("boogie");
+	/**
+	 * Base path to the Boogie resource folder.
+	 */
+	final private static Path boogiePath = resourcesPath.resolve("boogie");
 
-  /**
-   * Fetches the paths to the test Boogie files.
-   *
-   * @param bplName
-   *            The name of the Boogie file.
-   * @return The path to the Boogie file.
-   * @throws FileNotFoundException
-   *             If the resource could not be located.
-   */
-  public static Path getBoogiePath(final String bplName) throws FileNotFoundException {
-    final Path bplPath = boogiePath.resolve(bplName + ".bpl");
+	/**
+	 * Fetches the paths to the test Boogie files.
+	 *
+	 * @param bplName
+	 *            The name of the Boogie file.
+	 * @return The path to the Boogie file.
+	 * @throws FileNotFoundException
+	 *             If the resource could not be located.
+	 */
+	public static Path getBoogiePath(final String bplName) throws FileNotFoundException {
+		final Path bplPath = boogiePath.resolve(bplName + ".bpl");
 
-    if (Files.exists(bplPath)) {
-      return bplPath;
-    } else {
-      throw new FileNotFoundException("Could not find resource at " + bplPath.toString());
-    }
-  }
+		if (Files.exists(bplPath)) {
+			return bplPath;
+		} else {
+			throw new FileNotFoundException("Could not find resource at " + bplPath.toString());
+		}
+	}
 
-  /**
-   * Fetches the paths to the test Boogie files.
-   *
-   * @param bplName
-   *            The name of the Boogie file.
-   * @return The input stream of the Boogie file.
-   * @throws FileNotFoundException
-   *             If the resource could not be located.
-   */
-  public static Reader getBoogieReader(final String bplName) throws FileNotFoundException {
-    final Path bplPath = getBoogiePath(bplName);
-    final File bplFile = bplPath.toFile();
+	/**
+	 * Fetches the paths to the test Boogie files.
+	 *
+	 * @param bplName
+	 *            The name of the Boogie file.
+	 * @return The input stream of the Boogie file.
+	 * @throws FileNotFoundException
+	 *             If the resource could not be located.
+	 */
+	public static Reader getBoogieReader(final String bplName) throws FileNotFoundException {
+		final Path bplPath = getBoogiePath(bplName);
+		final File bplFile = bplPath.toFile();
 
-    return new FileReader(bplFile);
-  }
+		return new FileReader(bplFile);
+	}
 
 }
