byteback-frontend/boogie/src/test/java/byteback/frontend/boogie/ast/TypeDefinitionTest.java
@@ -2,9 +2,8 @@ package byteback.frontend.boogie.ast;
 
 import static org.junit.Assert.assertEquals;
 
-import org.junit.Test;
-
 import byteback.frontend.boogie.TestUtil;
+import org.junit.Test;
 
 public class TypeDefinitionTest extends ASTTestFixture {
 
@@ -26,12 +25,12 @@ public class TypeDefinitionTest extends ASTTestFixture {
 		typeDefinition.getDefinedType();
 	}
 
-  @Test
-  public void makeTypeAccess_OnSimpleUnitType_ReturnsExpectedTypeAccess() {
+	@Test
+	public void makeTypeAccess_OnSimpleUnitType_ReturnsExpectedTypeAccess() {
 		final TypeDefinition typeDefinition = getTypeDefinition("Simple", "Unit");
 		final TypeAccess actual = typeDefinition.getDefinedType().makeTypeAccess();
-    final TypeAccess expected = new UnknownTypeAccess(typeDefinition.getDefinedType().makeAccessor(), new List<>());
-    TestUtil.assertAstEquals(expected, actual);
-  }
+		final TypeAccess expected = new UnknownTypeAccess(typeDefinition.getDefinedType().makeAccessor(), new List<>());
+		TestUtil.assertAstEquals(expected, actual);
+	}
 
 }
