byteback-core/src/integration/resources/regression/java8/boogie/byteback.dummy.condition.Simple.bpl
@@ -1,12 +1,64 @@
+// -------------------------------------------------------------------
+// Heap model
+// -------------------------------------------------------------------
+type Reference;
+
+const ~null: Reference;
+
+type Field a;
+type Store = [Reference]<a>[Field a]a;
+
+var ~heap: Store;
+
+function ~read<a>(h: Store, r: Reference, f: Field a) returns (a)
+{ h[r][f] }
+
+function ~update<a>(h: Store, r: Reference, f: Field a, v: a) returns (Store)
+{ h[r := h[r][f := v]] }
+
+// -------------------------------------------------------------------
+// Binary operators
+// -------------------------------------------------------------------
+function ~cmp<a>(a, a) returns (int);
+
+axiom (forall i: int, j: int :: i < j ==> ~cmp(i, j) == -1);
+axiom (forall i: int, j: int :: i > j ==> ~cmp(i, j) == 1);
+axiom (forall i: int, j: int :: i == j ==> ~cmp(i, j) == 0);
+
+axiom (forall i: real, j: real :: i < j ==> ~cmp(i, j) == -1);
+axiom (forall i: real, j: real :: i > j ==> ~cmp(i, j) == 1);
+axiom (forall i: real, j: real :: i == j ==> ~cmp(i, j) == 0);
+
+// -------------------------------------------------------------------
+// Casting operators
+// -------------------------------------------------------------------
+
+// Casting between primitive types
+function ~int<a>(a) returns (int);
+
+// bool -> int
+axiom ~int(false) == 0;
+axiom ~int(true) == 1;
+
+function eq(~heap: Store, a: int, b: int) returns (bool) { a == b }
+
+// real -> int
+// TODO
+
+function ~real<a>(a) returns (real);
+
+// int -> real
+// TODO
+
 procedure byteback.dummy.condition.Simple.returnsOne##() returns (~ret: int)
-  ensures ~ret == 1;
+  ensures eq(~heap, ~ret, 1);
 {
   ~ret := 1;
   return;
 }
 
 procedure byteback.dummy.condition.Simple.identity#int#(a: int) returns (~ret: int)
-  ensures ~ret == a;
+  ensures eq(~heap, ~ret, a);
 {
   ~ret := a;
   return;
